LwRust/Paper/Examples/WhileJoinPass.lean
@@ -23,9 +23,11 @@ def whileJoinRetargetLoopExample : Term :=
       (.eq
         (.copy (.deref (.var "q")))    -- Rust: *q
         (.val (.int 0)))               -- Rust: == 0
-      (.assign
-        (.var "q")                     -- Rust: q
-        (.borrow false (.var "y")))    -- Rust: = &y;
+      (.block [0, 0, 0] [              -- Rust: {
+        .assign
+          (.var "q")                   -- Rust: q
+          (.borrow false (.var "y"))   -- Rust: = &y;
+      ])
   ]
 
 theorem whileJoinRetargetLoopExample_accepted :
